Specify functions in rest

src/proof/k8s_io/apimachinery/pkg/apis/meta/v1.v
@@ -5,143 +5,154 @@ Section proof.
 Context `{hG: !heapGS Σ} {go_ctx: GoContext}.
 
 Lemma wp_Now:
-  {{{ is_pkg_init code.k8s_io.apimachinery.pkg.apis.meta.v1.v1 }}}
+  {{{ is_pkg_init v1 }}}
     @! v1.Now #()
   {{{ (c: v1.Time.t) v, RET #c;
     TimeV.deepown c v
   }}}.
-Proof.
-Admitted.
+Proof. Admitted.
 
-Lemma wp_GetName (ptr: loc) (meta: v1.ObjectMeta.t):
-  {{{ is_pkg_init code.k8s_io.apimachinery.pkg.apis.meta.v1.v1 ∗
-      ptr ↦ meta
+Lemma wp_GetName l m :
+  {{{ is_pkg_init v1 ∗
+      l ↦ m
   }}}
-    ptr @ (ptrT.id v1.ObjectMeta.id) @ "GetName" #()
-  {{{ RET #meta.(v1.ObjectMeta.Name');
-      ptr ↦ meta
+    l @ (ptrT.id v1.ObjectMeta.id) @ "GetName" #()
+  {{{ RET #m.(v1.ObjectMeta.Name');
+      l ↦ m
   }}}.
-Proof.
-  wp_start as "H". iNamed "H". wp_auto. iApply "HΦ". iFrame.
-Qed.
+Proof. wp_start as "H". wp_auto. iApply "HΦ". iFrame. Qed.
 
-Lemma wp_GetGenerateName (ptr: loc) (meta: v1.ObjectMeta.t):
-  {{{ is_pkg_init code.k8s_io.apimachinery.pkg.apis.meta.v1.v1 ∗
-      ptr ↦ meta
+Lemma wp_SetName l m name :
+  {{{ is_pkg_init v1 ∗
+      l ↦ m
   }}}
-    ptr @ (ptrT.id v1.ObjectMeta.id) @ "GetGenerateName" #()
-  {{{ RET #meta.(v1.ObjectMeta.GenerateName');
-      ptr ↦ meta
-  }}}.
-Proof.
-  wp_start as "H". iNamed "H". wp_auto. iApply "HΦ". iFrame.
-Qed.
-
-Lemma wp_SetName (ptr: loc) (meta: v1.ObjectMeta.t) (name: go_string):
-  {{{ is_pkg_init code.k8s_io.apimachinery.pkg.apis.meta.v1.v1 ∗
-      ptr ↦ meta
-  }}}
-    ptr @ (ptrT.id v1.ObjectMeta.id) @ "SetName" #name
+    l @ (ptrT.id v1.ObjectMeta.id) @ "SetName" #name
   {{{ RET #();
-      ptr ↦ meta <| v1.ObjectMeta.Name' := name |>
+      l ↦ m <| v1.ObjectMeta.Name' := name |>
   }}}.
-Proof.
-  wp_start as "H". iNamed "H". wp_auto. iApply "HΦ". iFrame.
-Qed.
+Proof. wp_start as "H". wp_auto. iApply "HΦ". iFrame. Qed.
 
-Lemma wp_SetNamespace (ptr: loc) (meta: v1.ObjectMeta.t) (namespace: go_string):
-  {{{ is_pkg_init code.k8s_io.apimachinery.pkg.apis.meta.v1.v1 ∗
-      ptr ↦ meta
+Lemma wp_GetGenerateName l m :
+  {{{ is_pkg_init v1 ∗
+      l ↦ m
   }}}
-    ptr @ (ptrT.id v1.ObjectMeta.id) @ "SetNamespace" #namespace
+    l @ (ptrT.id v1.ObjectMeta.id) @ "GetGenerateName" #()
+  {{{ RET #m.(v1.ObjectMeta.GenerateName');
+      l ↦ m
+  }}}.
+Proof. wp_start as "H". wp_auto. iApply "HΦ". iFrame. Qed.
+
+Lemma wp_SetNamespace l m namespace :
+  {{{ is_pkg_init v1 ∗
+      l ↦ m
+  }}}
+    l @ (ptrT.id v1.ObjectMeta.id) @ "SetNamespace" #namespace
   {{{ RET #();
-      ptr ↦ meta <| v1.ObjectMeta.Namespace' := namespace |>
+      l ↦ m <| v1.ObjectMeta.Namespace' := namespace |>
   }}}.
-Proof.
-  wp_start as "H". iNamed "H". wp_auto. iApply "HΦ". iFrame.
-Qed.
+Proof. wp_start as "H". wp_auto. iApply "HΦ". iFrame. Qed.
 
-Lemma wp_GetDeletionTimestamp (ptr: loc) (meta: v1.ObjectMeta.t):
-  {{{ is_pkg_init code.k8s_io.apimachinery.pkg.apis.meta.v1.v1 ∗
-      ptr ↦ meta
+Lemma wp_SetCreationTimestamp l m creation_timestamp :
+  {{{ is_pkg_init v1 ∗
+      l ↦ m
   }}}
-    ptr @ (ptrT.id v1.ObjectMeta.id) @ "GetDeletionTimestamp" #()
-  {{{ RET #meta.(v1.ObjectMeta.DeletionTimestamp');
-      ptr ↦ meta
-  }}}.
-Proof.
-  wp_start as "H". iNamed "H". wp_auto. iApply "HΦ". iFrame.
-Qed.
-
-Lemma wp_SetDeletionTimestamp (ptr: loc) (meta: v1.ObjectMeta.t) (deletion_timestamp: loc):
-  {{{ is_pkg_init code.k8s_io.apimachinery.pkg.apis.meta.v1.v1 ∗
-      ptr ↦ meta
-  }}}
-    ptr @ (ptrT.id v1.ObjectMeta.id) @ "SetDeletionTimestamp" #deletion_timestamp
+    l @ (ptrT.id v1.ObjectMeta.id) @ "SetCreationTimestamp" #creation_timestamp
   {{{ RET #();
-      ptr ↦ meta <| v1.ObjectMeta.DeletionTimestamp' := deletion_timestamp |>
+      l ↦ m <| v1.ObjectMeta.CreationTimestamp' := creation_timestamp |>
   }}}.
-Proof.
-  wp_start as "H". iNamed "H". wp_auto. iApply "HΦ". iFrame.
-Qed.
+Proof. wp_start as "H". wp_auto. iApply "HΦ". iFrame. Qed.
 
-Lemma wp_SetResourceVersion (ptr: loc) (meta: v1.ObjectMeta.t) (resource_version: go_string):
-  {{{ is_pkg_init code.k8s_io.apimachinery.pkg.apis.meta.v1.v1 ∗
-      ptr ↦ meta
+Lemma wp_GetDeletionTimestamp l m :
+  {{{ is_pkg_init v1 ∗
+      l ↦ m
   }}}
-    ptr @ (ptrT.id v1.ObjectMeta.id) @ "SetResourceVersion" #resource_version
+    l @ (ptrT.id v1.ObjectMeta.id) @ "GetDeletionTimestamp" #()
+  {{{ RET #m.(v1.ObjectMeta.DeletionTimestamp');
+      l ↦ m
+  }}}.
+Proof. wp_start as "H". iNamed "H". wp_auto. iApply "HΦ". iFrame. Qed.
+
+Lemma wp_SetDeletionTimestamp l m deletion_timestamp :
+  {{{ is_pkg_init v1 ∗
+      l ↦ m
+  }}}
+    l @ (ptrT.id v1.ObjectMeta.id) @ "SetDeletionTimestamp" #deletion_timestamp
   {{{ RET #();
-      ptr ↦ meta <| v1.ObjectMeta.ResourceVersion' := resource_version |>
+      l ↦ m <| v1.ObjectMeta.DeletionTimestamp' := deletion_timestamp |>
   }}}.
-Proof.
-  wp_start as "H". iNamed "H". wp_auto. iApply "HΦ". iFrame.
-Qed.
+Proof. wp_start as "H". wp_auto. iApply "HΦ". iFrame. Qed.
 
-Lemma wp_GetFinalizers (ptr: loc) (meta: v1.ObjectMeta.t):
-  {{{ is_pkg_init code.k8s_io.apimachinery.pkg.apis.meta.v1.v1 ∗
-      ptr ↦ meta
+Lemma wp_SetDeletionGracePeriodSeconds l m deletion_grace_period_seconds :
+  {{{ is_pkg_init v1 ∗
+      l ↦ m
   }}}
-    ptr @ (ptrT.id v1.ObjectMeta.id) @ "GetFinalizers" #()
-  {{{ RET #meta.(v1.ObjectMeta.Finalizers');
-      ptr ↦ meta
-  }}}.
-Proof.
-  wp_start as "H". iNamed "H". wp_auto. iApply "HΦ". iFrame.
-Qed.
-
-Lemma wp_SetUID (ptr: loc) (meta: v1.ObjectMeta.t) (uid: go_string):
-  {{{ is_pkg_init code.k8s_io.apimachinery.pkg.apis.meta.v1.v1 ∗
-      ptr ↦ meta
-  }}}
-    ptr @ (ptrT.id v1.ObjectMeta.id) @ "SetUID" #uid
+    l @ (ptrT.id v1.ObjectMeta.id) @ "SetDeletionGracePeriodSeconds" #deletion_grace_period_seconds
   {{{ RET #();
-      ptr ↦ meta <| v1.ObjectMeta.UID' := uid |>
+      l ↦ m <| v1.ObjectMeta.DeletionGracePeriodSeconds' := deletion_grace_period_seconds |>
   }}}.
-Proof.
-  wp_start as "H". iNamed "H". wp_auto. iApply "HΦ". iFrame.
-Qed.
+Proof. wp_start as "H". wp_auto. iApply "HΦ". iFrame. Qed.
 
-Definition new_controller_ref_valid controller_ref kind meta: Prop :=
+Lemma wp_SetSelfLink l m self_link :
+  {{{ is_pkg_init v1 ∗
+      l ↦ m
+  }}}
+    l @ (ptrT.id v1.ObjectMeta.id) @ "SetSelfLink" #self_link
+  {{{ RET #();
+      l ↦ m <| v1.ObjectMeta.SelfLink' := self_link |>
+  }}}.
+Proof. wp_start as "H". wp_auto. iApply "HΦ". iFrame. Qed.
+
+Lemma wp_SetResourceVersion l m resource_version :
+  {{{ is_pkg_init v1 ∗
+      l ↦ m
+  }}}
+    l @ (ptrT.id v1.ObjectMeta.id) @ "SetResourceVersion" #resource_version
+  {{{ RET #();
+      l ↦ m <| v1.ObjectMeta.ResourceVersion' := resource_version |>
+  }}}.
+Proof. wp_start as "H". wp_auto. iApply "HΦ". iFrame. Qed.
+
+Lemma wp_GetFinalizers l m :
+  {{{ is_pkg_init v1 ∗
+      l ↦ m
+  }}}
+    l @ (ptrT.id v1.ObjectMeta.id) @ "GetFinalizers" #()
+  {{{ RET #m.(v1.ObjectMeta.Finalizers');
+      l ↦ m
+  }}}.
+Proof. wp_start as "H". wp_auto. iApply "HΦ". iFrame. Qed.
+
+Lemma wp_SetUID l m uid :
+  {{{ is_pkg_init v1 ∗
+      l ↦ m
+  }}}
+    l @ (ptrT.id v1.ObjectMeta.id) @ "SetUID" #uid
+  {{{ RET #();
+      l ↦ m <| v1.ObjectMeta.UID' := uid |>
+  }}}.
+Proof. wp_start as "H". wp_auto. iApply "HΦ". iFrame. Qed.
+
+Definition new_controller_ref_valid controller_ref kind m : Prop :=
   controller_ref.(OwnerReferenceV.Kind') = kind ∧
-  controller_ref.(OwnerReferenceV.Name') = meta.(ObjectMetaV.Name') ∧
-  controller_ref.(OwnerReferenceV.UID') = meta.(ObjectMetaV.UID') ∧
+  controller_ref.(OwnerReferenceV.Name') = m.(ObjectMetaV.Name') ∧
+  controller_ref.(OwnerReferenceV.UID') = m.(ObjectMetaV.UID') ∧
   controller_ref.(OwnerReferenceV.BlockOwnerDeletion') = Some true ∧
   controller_ref.(OwnerReferenceV.Controller') = Some true.
 
-Lemma wp_NewControllerRef_replicaset owner gvk rs_l meta pure_meta dq:
-  {{{ is_pkg_init code.k8s_io.apimachinery.pkg.apis.meta.v1.v1 ∗
+Lemma wp_NewControllerRef_replicaset owner gvk rs_l m pure_m dq:
+  {{{ is_pkg_init v1 ∗
       ⌜ owner = interface.mk (ptrT.id v1.ReplicaSet.id) (# rs_l) ⌝ ∗
-      rs_l ↦s[v1.ReplicaSet :: "ObjectMeta"]{dq} meta ∗
-      ObjectMetaV.deepown meta pure_meta dq
+      rs_l ↦s[v1.ReplicaSet :: "ObjectMeta"]{dq} m ∗
+      ObjectMetaV.deepown m pure_m dq
   }}}
     @! v1.NewControllerRef #owner #gvk
   {{{ l pure_controller_ref, RET #l;
       OwnerReferenceV.deepown_l l pure_controller_ref 1 ∗
-      ⌜ new_controller_ref_valid pure_controller_ref gvk.(schema.GroupVersionKind.Kind') pure_meta ⌝ ∗
-      rs_l ↦s[v1.ReplicaSet :: "ObjectMeta"]{dq} meta ∗
-      ObjectMetaV.deepown meta pure_meta dq
+      ⌜ new_controller_ref_valid pure_controller_ref gvk.(schema.GroupVersionKind.Kind') pure_m ⌝ ∗
+      rs_l ↦s[v1.ReplicaSet :: "ObjectMeta"]{dq} m ∗
+      ObjectMetaV.deepown m pure_m dq
   }}}.
-Proof. wp_start as "H". Admitted.
+Proof. Admitted.
 
 Definition namespace_matches ns_query ns: Prop :=
   ns_query = v1.NamespaceAll ∨ ns_query = ns.
