src/proof/k8s_io/apiserver/pkg/registry/rest.v
@@ -1,0 +1,45 @@
+From New.proof.k8s_io.apiserver.pkg.registry Require Export rest_init.
+From New.proof.k8s_io.apimachinery.pkg.apis.meta Require Export v1_init.
+From New.proof Require Import prelude empty_ffi pure_objects.
+
+Section proof.
+Context `{hG: !heapGS Σ} {go_ctx: GoContext}.
+
+Lemma wp_WipeObjectMetaSystemFields l m :
+  {{{ is_pkg_init rest ∗
+      l ↦ m
+  }}}
+    @! rest.WipeObjectMetaSystemFields #l
+  {{{ time, RET #();
+      l ↦ m <| v1.ObjectMeta.CreationTimestamp' := time |>
+            <| v1.ObjectMeta.UID' := ""%go |>
+            <| v1.ObjectMeta.DeletionTimestamp' := null |>
+            <| v1.ObjectMeta.DeletionGracePeriodSeconds' := null |>
+            <| v1.ObjectMeta.SelfLink' := ""%go |>
+  }}}.
+Proof. Admitted.
+
+Lemma wp_FillObjectMetaSystemFields l m :
+  {{{ is_pkg_init rest ∗
+      l ↦ m
+  }}}
+    @! rest.FillObjectMetaSystemFields #l
+  {{{ time timev uid, RET #();
+      l ↦ m <| v1.ObjectMeta.CreationTimestamp' := time |>
+            <| v1.ObjectMeta.UID' := uid |> ∗
+      TimeV.deepown time timev
+  }}}.
+Proof. Admitted.
+
+Lemma wp_EnsureObjectNamespaceMatchesRequestNamespace ns l m :
+  {{{ is_pkg_init rest ∗
+      l ↦ m ∗
+      ⌜ m.(v1.ObjectMeta.Namespace') = ""%go ∨ m.(v1.ObjectMeta.Namespace') = ns ⌝
+  }}}
+    @! rest.EnsureObjectNamespaceMatchesRequestNamespace #ns #l
+  {{{ RET #interface.nil;
+      l ↦ m <| v1.ObjectMeta.Namespace' := ns |>
+  }}}.
+Proof. Admitted.
+
+End proof.
